------------------------------------------------------------------------
-- The Agda standard library
--
-- Basic properties of ℕᵇ
------------------------------------------------------------------------

{-# OPTIONS --without-K --safe #-}

module Data.Nat.Binary.Properties where

open import Algebra.Bundles
open import Algebra.Morphism.Structures
import Algebra.Morphism.MonoidMonomorphism as MonoidMonomorphism
open import Algebra.Consequences.Propositional
open import Data.Nat.Binary.Base
open import Data.Nat as ℕ using (ℕ; z≤n; s≤s)
import Data.Nat.Properties as ℕₚ
open import Data.Nat.Solver
open import Data.Product using (_,_; proj₁; proj₂; ∃)
open import Data.Sum.Base using (_⊎_; inj₁; inj₂)
open import Function using (_∘_; _$_; id)
open import Function.Definitions using (Injective)
open import Function.Definitions.Core2 using (Surjective)
open import Level using (0ℓ)
open import Relation.Binary
open import Relation.Binary.Consequences
open import Relation.Binary.Morphism
import Relation.Binary.Morphism.OrderMonomorphism as OrderMonomorphism
open import Relation.Binary.PropositionalEquality
import Relation.Binary.Reasoning.Base.Triple as InequalityReasoning
open import Relation.Nullary using (¬_; yes; no)
import Relation.Nullary.Decidable as Dec
open import Relation.Nullary.Negation using (contradiction)

open import Algebra.Definitions {A = ℕᵇ} _≡_
open import Algebra.Structures {A = ℕᵇ} _≡_
import Algebra.Properties.CommutativeSemigroup as CommSemigProp
import Algebra.Properties.CommutativeSemigroup ℕₚ.+-commutativeSemigroup
  as ℕ-+-semigroupProperties
import Relation.Binary.Construct.StrictToNonStrict _≡_ _<_
  as StrictToNonStrict
open +-*-Solver

------------------------------------------------------------------------
-- Properties of _≡_
------------------------------------------------------------------------

2[1+x]≢0 : ∀ {x} → 2[1+ x ] ≢ 0ᵇ
2[1+x]≢0 ()

1+[2x]≢0 : ∀ {x} → 1+[2 x ] ≢ 0ᵇ
1+[2x]≢0 ()

2[1+_]-injective : Injective _≡_ _≡_ 2[1+_]
2[1+_]-injective refl = refl

1+[2_]-injective : Injective _≡_ _≡_ 1+[2_]
1+[2_]-injective refl = refl

_≟_ : Decidable {A = ℕᵇ} _≡_
zero     ≟ zero     =  yes refl
zero     ≟ 2[1+ _ ] =  no λ()
zero     ≟ 1+[2 _ ] =  no λ()
2[1+ _ ] ≟ zero     =  no λ()
2[1+ x ] ≟ 2[1+ y ] =  Dec.map′ (cong 2[1+_]) 2[1+_]-injective (x ≟ y)
2[1+ _ ] ≟ 1+[2 _ ] =  no λ()
1+[2 _ ] ≟ zero     =  no λ()
1+[2 _ ] ≟ 2[1+ _ ] =  no λ()
1+[2 x ] ≟ 1+[2 y ] =  Dec.map′ (cong 1+[2_]) 1+[2_]-injective (x ≟ y)

≡-isDecEquivalence : IsDecEquivalence {A = ℕᵇ} _≡_
≡-isDecEquivalence = isDecEquivalence _≟_

≡-setoid : Setoid 0ℓ 0ℓ
≡-setoid = setoid ℕᵇ

≡-decSetoid : DecSetoid 0ℓ 0ℓ
≡-decSetoid = decSetoid _≟_

------------------------------------------------------------------------
-- Properties of toℕ & fromℕ
------------------------------------------------------------------------

toℕ-double : ∀ x → toℕ (double x) ≡ 2 ℕ.* (toℕ x)
toℕ-double zero     =  refl
toℕ-double 1+[2 x ] =  cong ((2 ℕ.*_) ∘ ℕ.suc) (toℕ-double x)
toℕ-double 2[1+ x ] =  cong (2 ℕ.*_) (sym (ℕₚ.*-distribˡ-+ 2 1 (toℕ x)))

toℕ-suc : ∀ x → toℕ (suc x) ≡ ℕ.suc (toℕ x)
toℕ-suc zero     =  refl
toℕ-suc 2[1+ x ] =  cong (ℕ.suc ∘ (2 ℕ.*_)) (toℕ-suc x)
toℕ-suc 1+[2 x ] =  ℕₚ.*-distribˡ-+ 2 1 (toℕ x)

toℕ-pred : ∀ x → toℕ (pred x) ≡ ℕ.pred (toℕ x)
toℕ-pred zero     =  refl
toℕ-pred 2[1+ x ] =  cong ℕ.pred $ sym $ ℕₚ.*-distribˡ-+ 2 1 (toℕ x)
toℕ-pred 1+[2 x ] =  toℕ-double x

toℕ-fromℕ : toℕ ∘ fromℕ ≗ id
toℕ-fromℕ 0         = refl
toℕ-fromℕ (ℕ.suc n) = begin
  toℕ (fromℕ (ℕ.suc n))   ≡⟨⟩
  toℕ (suc (fromℕ n))     ≡⟨ toℕ-suc (fromℕ n) ⟩
  ℕ.suc (toℕ (fromℕ n))   ≡⟨ cong ℕ.suc (toℕ-fromℕ n) ⟩
  ℕ.suc n                 ∎
  where open ≡-Reasoning

toℕ-injective : Injective _≡_ _≡_ toℕ
toℕ-injective {zero}     {zero}     _               =  refl
toℕ-injective {2[1+ x ]} {2[1+ y ]} 2[1+xN]≡2[1+yN] =  cong 2[1+_] x≡y
  where
  1+xN≡1+yN = ℕₚ.*-cancelˡ-≡ {ℕ.suc _} {ℕ.suc _} 1 2[1+xN]≡2[1+yN]
  xN≡yN     = cong ℕ.pred 1+xN≡1+yN
  x≡y       = toℕ-injective xN≡yN

toℕ-injective {2[1+ x ]} {1+[2 y ]} 2[1+xN]≡1+2yN =
  contradiction 2[1+xN]≡1+2yN (ℕₚ.even≢odd (ℕ.suc (toℕ x)) (toℕ y))

toℕ-injective {1+[2 x ]} {2[1+ y ]} 1+2xN≡2[1+yN] =
  contradiction (sym 1+2xN≡2[1+yN]) (ℕₚ.even≢odd (ℕ.suc (toℕ y)) (toℕ x))

toℕ-injective {1+[2 x ]} {1+[2 y ]} 1+2xN≡1+2yN =  cong 1+[2_] x≡y
  where
  2xN≡2yN = cong ℕ.pred 1+2xN≡1+2yN
  xN≡yN   = ℕₚ.*-cancelˡ-≡ 1 2xN≡2yN
  x≡y     = toℕ-injective xN≡yN

toℕ-surjective : Surjective _≡_ toℕ
toℕ-surjective n = (fromℕ n , toℕ-fromℕ n)

toℕ-isRelHomomorphism : IsRelHomomorphism _≡_ _≡_ toℕ
toℕ-isRelHomomorphism = record
  { cong = cong toℕ
  }

fromℕ-injective : Injective _≡_ _≡_ fromℕ
fromℕ-injective {x} {y} f[x]≡f[y] = begin
  x             ≡⟨ sym (toℕ-fromℕ x) ⟩
  toℕ (fromℕ x) ≡⟨ cong toℕ f[x]≡f[y] ⟩
  toℕ (fromℕ y) ≡⟨ toℕ-fromℕ y ⟩
  y             ∎
  where open ≡-Reasoning

fromℕ-toℕ : fromℕ ∘ toℕ ≗ id
fromℕ-toℕ =  toℕ-injective ∘ toℕ-fromℕ ∘ toℕ

fromℕ-pred : ∀ n → fromℕ (ℕ.pred n) ≡ pred (fromℕ n)
fromℕ-pred n = begin
  fromℕ (ℕ.pred n)        ≡⟨ cong (fromℕ ∘ ℕ.pred) (sym (toℕ-fromℕ n)) ⟩
  fromℕ (ℕ.pred (toℕ x))  ≡⟨ cong fromℕ (sym (toℕ-pred x)) ⟩
  fromℕ (toℕ (pred x))    ≡⟨ fromℕ-toℕ (pred x) ⟩
  pred x                  ≡⟨ refl ⟩
  pred (fromℕ n)          ∎
  where open ≡-Reasoning;  x = fromℕ n

x≡0⇒toℕ[x]≡0 : ∀ {x} → x ≡ zero → toℕ x ≡ 0
x≡0⇒toℕ[x]≡0 {zero} _ = refl

toℕ[x]≡0⇒x≡0 : ∀ {x} → toℕ x ≡ 0 → x ≡ zero
toℕ[x]≡0⇒x≡0 {zero} _ = refl

------------------------------------------------------------------------
-- Properties of _<_
------------------------------------------------------------------------
-- Basic properties

x≮0 : ∀ {x} → x ≮ zero
x≮0 ()

x≢0⇒x>0 : ∀ {x} → x ≢ zero → x > zero
x≢0⇒x>0 {zero}     0≢0 =  contradiction refl 0≢0
x≢0⇒x>0 {2[1+ _ ]} _   =  0<even
x≢0⇒x>0 {1+[2 _ ]} _   =  0<odd

1+[2x]<2[1+x] : ∀ x → 1+[2 x ] < 2[1+ x ]
1+[2x]<2[1+x] x =  odd<even (inj₂ refl)

<⇒≢ : _<_ ⇒ _≢_
<⇒≢ (even<even x<x) refl = <⇒≢ x<x refl
<⇒≢ (odd<odd   x<x) refl = <⇒≢ x<x refl

>⇒≢ : _>_ ⇒ _≢_
>⇒≢ y<x =  ≢-sym (<⇒≢ y<x)

≡⇒≮ : _≡_ ⇒ _≮_
≡⇒≮ x≡y x<y =  <⇒≢ x<y x≡y

≡⇒≯ : _≡_ ⇒ _≯_
≡⇒≯ x≡y x>y =  >⇒≢ x>y x≡y

<⇒≯ : _<_ ⇒ _≯_
<⇒≯ (even<even x<y)        (even<even y<x)        = <⇒≯ x<y y<x
<⇒≯ (even<odd x<y)         (odd<even (inj₁ y<x))  = <⇒≯ x<y y<x
<⇒≯ (even<odd x<y)         (odd<even (inj₂ refl)) = <⇒≢ x<y refl
<⇒≯ (odd<even (inj₁ x<y))  (even<odd y<x)         = <⇒≯ x<y y<x
<⇒≯ (odd<even (inj₂ refl)) (even<odd y<x)         = <⇒≢ y<x refl
<⇒≯ (odd<odd x<y)          (odd<odd y<x)          = <⇒≯ x<y y<x

>⇒≮ : _>_ ⇒ _≮_
>⇒≮ y<x =  <⇒≯ y<x

<⇒≤ : _<_ ⇒ _≤_
<⇒≤ = inj₁

------------------------------------------------------------------------------
-- Properties of _<_ and toℕ & fromℕ.

toℕ-mono-< : toℕ Preserves _<_ ⟶ ℕ._<_
toℕ-mono-< {zero}     {2[1+ _ ]} _               =  ℕₚ.0<1+n
toℕ-mono-< {zero}     {1+[2 _ ]} _               =  ℕₚ.0<1+n
toℕ-mono-< {2[1+ x ]} {2[1+ y ]} (even<even x<y) =  begin
  ℕ.suc (2 ℕ.* (ℕ.suc xN))    ≤⟨ ℕₚ.+-monoʳ-≤ 1 (ℕₚ.*-monoʳ-≤ 2 xN<yN) ⟩
  ℕ.suc (2 ℕ.* yN)            ≤⟨ ℕₚ.≤-step ℕₚ.≤-refl ⟩
  2 ℕ.+ (2 ℕ.* yN)            ≡⟨ sym (ℕₚ.*-distribˡ-+ 2 1 yN) ⟩
  2 ℕ.* (ℕ.suc yN)            ∎
  where open ℕₚ.≤-Reasoning;  xN = toℕ x;  yN = toℕ y;  xN<yN = toℕ-mono-< x<y
toℕ-mono-< {2[1+ x ]} {1+[2 y ]} (even<odd x<y) =
  ℕₚ.+-monoʳ-≤ 1 (ℕₚ.*-monoʳ-≤ 2 (toℕ-mono-< x<y))
toℕ-mono-< {1+[2 x ]} {2[1+ y ]} (odd<even (inj₁ x<y)) =   begin
  ℕ.suc (ℕ.suc (2 ℕ.* xN))    ≡⟨⟩
  2 ℕ.+ (2 ℕ.* xN)            ≡⟨ sym (ℕₚ.*-distribˡ-+ 2 1 xN) ⟩
  2 ℕ.* (ℕ.suc xN)            ≤⟨ ℕₚ.*-monoʳ-≤ 2 xN<yN ⟩
  2 ℕ.* yN                    ≤⟨ ℕₚ.*-monoʳ-≤ 2 (ℕₚ.≤-step ℕₚ.≤-refl) ⟩
  2 ℕ.* (ℕ.suc yN)            ∎
  where open ℕₚ.≤-Reasoning;  xN = toℕ x;  yN = toℕ y;  xN<yN = toℕ-mono-< x<y
toℕ-mono-< {1+[2 x ]} {2[1+ .x ]} (odd<even (inj₂ refl)) =
  ℕₚ.≤-reflexive (sym (ℕₚ.*-distribˡ-+ 2 1 (toℕ x)))
toℕ-mono-< {1+[2 x ]} {1+[2 y ]} (odd<odd x<y) =  ℕₚ.+-monoʳ-< 1 (ℕₚ.*-monoʳ-< 1 xN<yN)
  where xN = toℕ x;  yN = toℕ y;  xN<yN = toℕ-mono-< x<y

toℕ-cancel-< : ∀ {x y} → toℕ x ℕ.< toℕ y → x < y
toℕ-cancel-< {zero}     {2[1+ y ]} x<y = 0<even
toℕ-cancel-< {zero}     {1+[2 y ]} x<y = 0<odd
toℕ-cancel-< {2[1+ x ]} {2[1+ y ]} x<y =
  even<even (toℕ-cancel-< (ℕ.≤-pred (ℕₚ.*-cancelˡ-< 2 x<y)))
toℕ-cancel-< {2[1+ x ]} {1+[2 y ]} x<y
  rewrite ℕₚ.*-distribˡ-+ 2 1 (toℕ x) =
  even<odd (toℕ-cancel-< (ℕₚ.*-cancelˡ-< 2 (ℕₚ.≤-trans (s≤s (ℕₚ.n≤1+n _)) (ℕₚ.≤-pred x<y))))
toℕ-cancel-< {1+[2 x ]} {2[1+ y ]} x<y with toℕ x ℕₚ.≟ toℕ y
... | yes x≡y = odd<even (inj₂ (toℕ-injective x≡y))
... | no  x≢y
  rewrite ℕₚ.+-suc (toℕ y) (toℕ y ℕ.+ 0) =
  odd<even (inj₁ (toℕ-cancel-< (ℕₚ.≤∧≢⇒< (ℕₚ.*-cancelˡ-≤ 1 (ℕₚ.+-cancelˡ-≤ 2 x<y)) x≢y)))
toℕ-cancel-< {1+[2 x ]} {1+[2 y ]} x<y =
  odd<odd (toℕ-cancel-< (ℕₚ.*-cancelˡ-< 2 (ℕ.≤-pred x<y)))

fromℕ-cancel-< : ∀ {x y} → fromℕ x < fromℕ y → x ℕ.< y
fromℕ-cancel-< = subst₂ ℕ._<_ (toℕ-fromℕ _) (toℕ-fromℕ _) ∘ toℕ-mono-<

fromℕ-mono-< : fromℕ Preserves ℕ._<_ ⟶ _<_
fromℕ-mono-< = toℕ-cancel-< ∘ subst₂ ℕ._<_ (sym (toℕ-fromℕ _)) (sym (toℕ-fromℕ _))

toℕ-isHomomorphism-< : IsOrderHomomorphism _≡_ _≡_ _<_ ℕ._<_ toℕ
toℕ-isHomomorphism-< = record
  { cong = cong toℕ
  ; mono = toℕ-mono-<
  }

toℕ-isMonomorphism-< : IsOrderMonomorphism _≡_ _≡_ _<_ ℕ._<_ toℕ
toℕ-isMonomorphism-< = record
  { isOrderHomomorphism = toℕ-isHomomorphism-<
  ; injective           = toℕ-injective
  ; cancel              = toℕ-cancel-<
  }

------------------------------------------------------------------------------
-- Relational properties of _<_

<-irrefl : Irreflexive _≡_ _<_
<-irrefl refl (even<even x<x) =  <-irrefl refl x<x
<-irrefl refl (odd<odd x<x)   =  <-irrefl refl x<x

<-trans : Transitive _<_
<-trans {zero} {_}      {2[1+ _ ]} _  _        =  0<even
<-trans {zero} {_}      {1+[2 _ ]} _  _        =  0<odd
<-trans (even<even x<y) (even<even y<z)        =  even<even (<-trans x<y y<z)
<-trans (even<even x<y) (even<odd y<z)         =  even<odd (<-trans x<y y<z)
<-trans (even<odd x<y)  (odd<even (inj₁ y<z))  =  even<even (<-trans x<y y<z)
<-trans (even<odd x<y)  (odd<even (inj₂ refl)) =  even<even x<y
<-trans (even<odd x<y)  (odd<odd y<z)          =  even<odd (<-trans x<y y<z)
<-trans (odd<even (inj₁ x<y))  (even<even y<z) =  odd<even (inj₁ (<-trans x<y y<z))
<-trans (odd<even (inj₂ refl)) (even<even x<z) =  odd<even (inj₁ x<z)
<-trans (odd<even (inj₁ x<y))  (even<odd y<z)  =  odd<odd (<-trans x<y y<z)
<-trans (odd<even (inj₂ refl)) (even<odd x<z)  =  odd<odd x<z
<-trans (odd<odd x<y) (odd<even (inj₁ y<z))    =  odd<even (inj₁ (<-trans x<y y<z))
<-trans (odd<odd x<y) (odd<even (inj₂ refl))   =  odd<even (inj₁ x<y)
<-trans (odd<odd x<y) (odd<odd y<z)            =  odd<odd (<-trans x<y y<z)

-- Should not be implemented via the morphism `toℕ` in order to
-- preserve O(log n) time requirement.
<-cmp : Trichotomous _≡_ _<_
<-cmp zero     zero      = tri≈ x≮0    refl  x≮0
<-cmp zero     2[1+ _ ]  = tri< 0<even (λ()) x≮0
<-cmp zero     1+[2 _ ]  = tri< 0<odd  (λ()) x≮0
<-cmp 2[1+ _ ] zero      = tri> (λ())  (λ()) 0<even
<-cmp 2[1+ x ] 2[1+ y ]  with <-cmp x y
... | tri< x<y _    _   =  tri< lt (<⇒≢ lt) (<⇒≯ lt)  where lt = even<even x<y
... | tri≈ _   refl _   =  tri≈ (<-irrefl refl) refl (<-irrefl refl)
... | tri> _   _    x>y =  tri> (>⇒≮ gt) (>⇒≢ gt) gt  where gt = even<even x>y
<-cmp 2[1+ x ] 1+[2 y ]  with <-cmp x y
... | tri< x<y _    _ =  tri< lt (<⇒≢ lt) (<⇒≯ lt)  where lt = even<odd x<y
... | tri≈ _   refl _ =  tri> (>⇒≮ gt) (>⇒≢ gt) gt
  where
  gt = subst (_< 2[1+ x ]) refl (1+[2x]<2[1+x] x)
... | tri> _ _ y<x =  tri> (>⇒≮ gt) (>⇒≢ gt) gt  where gt = odd<even (inj₁ y<x)
<-cmp 1+[2 _ ] zero =  tri> (>⇒≮ gt) (>⇒≢ gt) gt  where gt = 0<odd
<-cmp 1+[2 x ] 2[1+ y ]  with <-cmp x y
... | tri< x<y _ _ =  tri< lt (<⇒≢ lt) (<⇒≯ lt)  where lt = odd<even (inj₁ x<y)
... | tri≈ _ x≡y _ =  tri< lt (<⇒≢ lt) (<⇒≯ lt)  where lt = odd<even (inj₂ x≡y)
... | tri> _ _ x>y =  tri> (>⇒≮ gt) (>⇒≢ gt) gt  where gt = even<odd x>y
<-cmp 1+[2 x ] 1+[2 y ]  with <-cmp x y
... | tri< x<y _  _   =  tri< lt (<⇒≢ lt) (<⇒≯ lt)  where lt = odd<odd x<y
... | tri≈ _ refl _   =  tri≈ (≡⇒≮ refl) refl (≡⇒≯ refl)
... | tri> _ _    x>y =  tri> (>⇒≮ gt) (>⇒≢ gt) gt  where gt = odd<odd x>y

_<?_ : Decidable _<_
_<?_ = tri⟶dec< <-cmp

------------------------------------------------------------------------------
-- Structures for _<_

<-isStrictPartialOrder : IsStrictPartialOrder _≡_ _<_
<-isStrictPartialOrder = record
  { isEquivalence = isEquivalence
  ; irrefl        = <-irrefl
  ; trans         = <-trans
  ; <-resp-≈      = resp₂ _<_
  }

<-isStrictTotalOrder : IsStrictTotalOrder _≡_ _<_
<-isStrictTotalOrder = record
  { isEquivalence = isEquivalence
  ; trans         = <-trans
  ; compare       = <-cmp
  }

------------------------------------------------------------------------------
-- Bundles for _<_

<-strictPartialOrder : StrictPartialOrder _ _ _
<-strictPartialOrder = record
  { isStrictPartialOrder = <-isStrictPartialOrder
  }

<-strictTotalOrder : StrictTotalOrder _ _ _
<-strictTotalOrder = record
  { isStrictTotalOrder =  <-isStrictTotalOrder
  }

------------------------------------------------------------------------------
-- Other properties of _<_

x<2[1+x] : ∀ x → x < 2[1+ x ]
x<1+[2x] : ∀ x → x < 1+[2 x ]

x<2[1+x] zero     = 0<even
x<2[1+x] 2[1+ x ] = even<even (x<2[1+x] x)
x<2[1+x] 1+[2 x ] = odd<even (inj₁ (x<1+[2x] x))

x<1+[2x] zero     = 0<odd
x<1+[2x] 2[1+ x ] = even<odd (x<2[1+x] x)
x<1+[2x] 1+[2 x ] = odd<odd (x<1+[2x] x)

------------------------------------------------------------------------------
-- Properties of _≤_
------------------------------------------------------------------------------
-- Basic properties

<⇒≱ : _<_ ⇒ _≱_
<⇒≱ x<y (inj₁ y<x) =  contradiction y<x (<⇒≯ x<y)
<⇒≱ x<y (inj₂ y≡x) =  contradiction (sym y≡x) (<⇒≢ x<y)

≤⇒≯ : _≤_ ⇒ _≯_
≤⇒≯ x≤y x>y =  <⇒≱ x>y x≤y

≮⇒≥ : _≮_ ⇒ _≥_
≮⇒≥ {x} {y} x≮y  with <-cmp x y
... | tri< lt _  _   =  contradiction lt x≮y
... | tri≈ _  eq _   =  inj₂ (sym eq)
... | tri> _  _  y<x =  <⇒≤ y<x

≰⇒> : _≰_ ⇒ _>_
≰⇒> {x} {y} x≰y  with <-cmp x y
... | tri< lt _  _   =  contradiction (<⇒≤ lt) x≰y
... | tri≈ _  eq _   =  contradiction (inj₂ eq) x≰y
... | tri> _  _  x>y =  x>y

≤∧≢⇒< : ∀ {x y} → x ≤ y → x ≢ y → x < y
≤∧≢⇒< (inj₁ x<y) _   =  x<y
≤∧≢⇒< (inj₂ x≡y) x≢y =  contradiction x≡y x≢y

0≤x : ∀ x → zero ≤ x
0≤x zero     =  inj₂ refl
0≤x 2[1+ _ ] =  inj₁ 0<even
0≤x 1+[2 x ] =  inj₁ 0<odd

x≤0⇒x≡0 : ∀ {x} → x ≤ zero → x ≡ zero
x≤0⇒x≡0 (inj₂ x≡0) = x≡0

------------------------------------------------------------------------------
-- Properties of _<_ and toℕ & fromℕ.

fromℕ-mono-≤ : fromℕ Preserves ℕ._≤_ ⟶ _≤_
fromℕ-mono-≤ m≤n  with ℕₚ.m≤n⇒m<n∨m≡n m≤n
... | inj₁ m<n =  inj₁ (fromℕ-mono-< m<n)
... | inj₂ m≡n =  inj₂ (cong fromℕ m≡n)

toℕ-mono-≤ : toℕ Preserves _≤_ ⟶ ℕ._≤_
toℕ-mono-≤ (inj₁ x<y)  =  ℕₚ.<⇒≤ (toℕ-mono-< x<y)
toℕ-mono-≤ (inj₂ refl) =  ℕₚ.≤-reflexive refl

toℕ-cancel-≤ : ∀ {x y} → toℕ x ℕ.≤ toℕ y → x ≤ y
toℕ-cancel-≤ = subst₂ _≤_ (fromℕ-toℕ _) (fromℕ-toℕ _) ∘ fromℕ-mono-≤

fromℕ-cancel-≤ : ∀ {x y} → fromℕ x ≤ fromℕ y → x ℕ.≤ y
fromℕ-cancel-≤ = subst₂ ℕ._≤_ (toℕ-fromℕ _) (toℕ-fromℕ _) ∘ toℕ-mono-≤

toℕ-isHomomorphism-≤ : IsOrderHomomorphism _≡_ _≡_ _≤_ ℕ._≤_ toℕ
toℕ-isHomomorphism-≤ = record
  { cong = cong toℕ
  ; mono = toℕ-mono-≤
  }

toℕ-isMonomorphism-≤ : IsOrderMonomorphism _≡_ _≡_ _≤_ ℕ._≤_ toℕ
toℕ-isMonomorphism-≤ = record
  { isOrderHomomorphism = toℕ-isHomomorphism-≤
  ; injective           = toℕ-injective
  ; cancel              = toℕ-cancel-≤
  }

------------------------------------------------------------------------------
-- Relational properties of _≤_

≤-refl : Reflexive _≤_
≤-refl =  inj₂ refl

≤-reflexive : _≡_ ⇒ _≤_
≤-reflexive {x} {_} refl =  ≤-refl {x}

≤-trans : Transitive _≤_
≤-trans = StrictToNonStrict.trans isEquivalence (resp₂ _<_) <-trans

<-≤-trans : ∀ {x y z} → x < y → y ≤ z → x < z
<-≤-trans x<y (inj₁ y<z)  =  <-trans x<y y<z
<-≤-trans x<y (inj₂ refl) =  x<y

≤-<-trans : ∀ {x y z} → x ≤ y → y < z → x < z
≤-<-trans (inj₁ x<y)  y<z =  <-trans x<y y<z
≤-<-trans (inj₂ refl) y<z =  y<z

≤-antisym : Antisymmetric _≡_ _≤_
≤-antisym = StrictToNonStrict.antisym isEquivalence <-trans <-irrefl

≤-total : Total _≤_
≤-total x y with <-cmp x y
... | tri< x<y _  _   = inj₁ (<⇒≤ x<y)
... | tri≈ _  x≡y _   = inj₁ (≤-reflexive x≡y)
... | tri> _  _   y<x = inj₂ (<⇒≤ y<x)

-- Should not be implemented via the morphism `toℕ` in order to
-- preserve O(log n) time requirement.
_≤?_ : Decidable _≤_
x ≤? y with <-cmp x y
... | tri< x<y _   _   = yes (<⇒≤ x<y)
... | tri≈ _   x≡y _   = yes (≤-reflexive x≡y)
... | tri> _   _   y<x = no (<⇒≱ y<x)


------------------------------------------------------------------------------
-- Structures

≤-isPreorder : IsPreorder _≡_ _≤_
≤-isPreorder = record
  { isEquivalence = isEquivalence
  ; reflexive     = ≤-reflexive
  ; trans         = ≤-trans
  }

≤-isPartialOrder : IsPartialOrder _≡_ _≤_
≤-isPartialOrder = record
  { isPreorder = ≤-isPreorder
  ; antisym    = ≤-antisym
  }

≤-isTotalOrder : IsTotalOrder _≡_ _≤_
≤-isTotalOrder = record
  { isPartialOrder = ≤-isPartialOrder
  ; total          = ≤-total
  }

≤-isDecTotalOrder : IsDecTotalOrder _≡_ _≤_
≤-isDecTotalOrder = record
  { isTotalOrder = ≤-isTotalOrder
  ; _≟_          = _≟_
  ; _≤?_         = _≤?_
  }

------------------------------------------------------------------------------
-- Bundles

≤-preorder : Preorder 0ℓ 0ℓ 0ℓ
≤-preorder = record
  { isPreorder = ≤-isPreorder
  }

≤-partialOrder : Poset 0ℓ 0ℓ 0ℓ
≤-partialOrder = record
  { isPartialOrder = ≤-isPartialOrder
  }

≤-totalOrder : TotalOrder 0ℓ 0ℓ 0ℓ
≤-totalOrder = record
  { isTotalOrder = ≤-isTotalOrder
  }

≤-decTotalOrder : DecTotalOrder 0ℓ 0ℓ 0ℓ
≤-decTotalOrder = record
  { isDecTotalOrder = ≤-isDecTotalOrder
  }

------------------------------------------------------------------------------
-- Equational reasoning for _≤_ and _<_

module ≤-Reasoning = InequalityReasoning
  ≤-isPreorder
  <-trans
  (resp₂ _<_) <⇒≤
  <-≤-trans ≤-<-trans
  hiding (step-≈; step-≈˘)

------------------------------------------------------------------------------
-- Properties of _<ℕ_
------------------------------------------------------------------------------

<⇒<ℕ : ∀ {x y} → x < y → x <ℕ y
<⇒<ℕ x<y = toℕ-mono-< x<y

<ℕ⇒< : ∀ {x y} → x <ℕ y → x < y
<ℕ⇒< {x} {y} t[x]<t[y] = begin-strict
  x             ≡⟨ sym (fromℕ-toℕ x) ⟩
  fromℕ (toℕ x) <⟨ fromℕ-mono-< t[x]<t[y] ⟩
  fromℕ (toℕ y) ≡⟨ fromℕ-toℕ y ⟩
  y             ∎
  where open ≤-Reasoning

------------------------------------------------------------------------
-- Properties of _+_
------------------------------------------------------------------------

------------------------------------------------------------------------
-- Raw bundles for _+_

+-rawMagma : RawMagma 0ℓ 0ℓ
+-rawMagma = record
  { _≈_ = _≡_
  ; _∙_ = _+_
  }

+-0-rawMonoid : RawMonoid 0ℓ 0ℓ
+-0-rawMonoid = record
  { _≈_ = _≡_
  ; _∙_ = _+_
  ; ε   = 0ᵇ
  }

------------------------------------------------------------------------
-- toℕ/fromℕ are homomorphisms for _+_

toℕ-homo-+ : ∀ x y → toℕ (x + y) ≡ toℕ x ℕ.+ toℕ y
toℕ-homo-+ zero     _        = refl
toℕ-homo-+ 2[1+ x ] zero     = cong ℕ.suc (sym (ℕₚ.+-identityʳ _))
toℕ-homo-+ 1+[2 x ] zero     = cong ℕ.suc (sym (ℕₚ.+-identityʳ _))
toℕ-homo-+ 2[1+ x ] 2[1+ y ] = begin
  toℕ (2[1+ x ] + 2[1+ y ])          ≡⟨⟩
  toℕ 2[1+ (suc (x + y)) ]           ≡⟨⟩
  2 ℕ.* (1 ℕ.+ (toℕ (suc (x + y))))  ≡⟨ cong ((2 ℕ.*_) ∘ ℕ.suc) (toℕ-suc (x + y)) ⟩
  2 ℕ.* (2 ℕ.+ toℕ (x + y))          ≡⟨ cong ((2 ℕ.*_) ∘ (2 ℕ.+_)) (toℕ-homo-+ x y) ⟩
  2 ℕ.* (2 ℕ.+ (toℕ x ℕ.+ toℕ y))    ≡⟨ solve 2 (λ m n → con 2 :* (con 2 :+ (m :+ n))  :=
                                          con 2 :* (con 1 :+ m) :+ con 2 :* (con 1 :+ n))
                                          refl (toℕ x) (toℕ y) ⟩
  toℕ 2[1+ x ] ℕ.+ toℕ 2[1+ y ]      ∎
  where open ≡-Reasoning

toℕ-homo-+ 2[1+ x ] 1+[2 y ] = begin
  toℕ (2[1+ x ] + 1+[2 y ])             ≡⟨⟩
  toℕ (suc 2[1+ (x + y) ])              ≡⟨ toℕ-suc 2[1+ (x + y) ] ⟩
  ℕ.suc (toℕ 2[1+ (x + y) ])            ≡⟨⟩
  ℕ.suc (2 ℕ.* (ℕ.suc (toℕ (x + y))))   ≡⟨ cong (λ v → ℕ.suc (2 ℕ.* ℕ.suc v)) (toℕ-homo-+ x y) ⟩
  ℕ.suc (2 ℕ.* (ℕ.suc (m ℕ.+ n)))       ≡⟨ solve 2 (λ m n → con 1 :+ (con 2 :* (con 1 :+ (m :+ n))) :=
                                             con 2 :* (con 1 :+ m) :+ (con 1 :+ (con 2 :* n)))
                                             refl m n ⟩
  (2 ℕ.* ℕ.suc m) ℕ.+ (ℕ.suc (2 ℕ.* n)) ≡⟨⟩
  toℕ 2[1+ x ] ℕ.+ toℕ 1+[2 y ]         ∎
  where open ≡-Reasoning;  m = toℕ x; n = toℕ y

toℕ-homo-+ 1+[2 x ] 2[1+ y ] = begin
  toℕ (1+[2 x ] + 2[1+ y ])                 ≡⟨⟩
  toℕ (suc 2[1+ (x + y) ])                  ≡⟨ toℕ-suc 2[1+ (x + y) ] ⟩
  ℕ.suc (toℕ 2[1+ (x + y) ])                ≡⟨⟩
  ℕ.suc (2 ℕ.* (ℕ.suc (toℕ (x + y))))       ≡⟨ cong (ℕ.suc ∘ (2 ℕ.*_) ∘ ℕ.suc) (toℕ-homo-+ x y) ⟩
  ℕ.suc (2 ℕ.* (ℕ.suc (m ℕ.+ n)))           ≡⟨ solve 2 (λ m n → con 1 :+ (con 2 :* (con 1 :+ (m :+ n))) :=
                                                 (con 1 :+ (con 2 :* m)) :+ (con 2 :* (con 1 :+ n)))
                                                 refl m n ⟩
  (ℕ.suc (2 ℕ.* m)) ℕ.+ (2 ℕ.* (ℕ.suc n))   ≡⟨⟩
  toℕ 1+[2 x ] ℕ.+ toℕ 2[1+ y ]             ∎
  where open ≡-Reasoning;  m = toℕ x;  n = toℕ y

toℕ-homo-+ 1+[2 x ] 1+[2 y ] = begin
  toℕ (1+[2 x ] + 1+[2 y ])               ≡⟨⟩
  toℕ (suc 1+[2 (x + y) ])                ≡⟨ toℕ-suc 1+[2 (x + y) ] ⟩
  ℕ.suc (toℕ 1+[2 (x + y) ])              ≡⟨⟩
  ℕ.suc (ℕ.suc (2 ℕ.* (toℕ (x + y))))     ≡⟨ cong (ℕ.suc ∘ ℕ.suc ∘ (2 ℕ.*_)) (toℕ-homo-+ x y) ⟩
  ℕ.suc (ℕ.suc (2 ℕ.* (m ℕ.+ n)))         ≡⟨ solve 2 (λ m n → con 1 :+ (con 1 :+ (con 2 :* (m :+ n))) :=
                                               (con 1 :+ (con 2 :* m)) :+ (con 1 :+ (con 2 :* n)))
                                               refl m n ⟩
  (ℕ.suc (2 ℕ.* m)) ℕ.+ (ℕ.suc (2 ℕ.* n)) ≡⟨⟩
  toℕ 1+[2 x ] ℕ.+ toℕ 1+[2 y ]           ∎
  where open ≡-Reasoning;  m = toℕ x;  n = toℕ y

toℕ-isMagmaHomomorphism-+ : IsMagmaHomomorphism +-rawMagma ℕₚ.+-rawMagma toℕ
toℕ-isMagmaHomomorphism-+ = record
  { isRelHomomorphism = toℕ-isRelHomomorphism
  ; homo              = toℕ-homo-+
  }

toℕ-isMonoidHomomorphism-+ : IsMonoidHomomorphism +-0-rawMonoid ℕₚ.+-0-rawMonoid toℕ
toℕ-isMonoidHomomorphism-+ = record
  { isMagmaHomomorphism = toℕ-isMagmaHomomorphism-+
  ; ε-homo              = refl
  }

toℕ-isMonoidMonomorphism-+ : IsMonoidMonomorphism +-0-rawMonoid ℕₚ.+-0-rawMonoid toℕ
toℕ-isMonoidMonomorphism-+ = record
  { isMonoidHomomorphism = toℕ-isMonoidHomomorphism-+
  ; injective            = toℕ-injective
  }

suc≗1+ : suc ≗ 1ᵇ +_
suc≗1+ zero     = refl
suc≗1+ 2[1+ _ ] = refl
suc≗1+ 1+[2 _ ] = refl

suc-+ : ∀ x y → suc x + y ≡ suc (x + y)
suc-+ zero        y     =  sym (suc≗1+ y)
suc-+ 2[1+ x ] zero     =  refl
suc-+ 1+[2 x ] zero     =  refl
suc-+ 2[1+ x ] 2[1+ y ] =  cong (suc ∘ 2[1+_]) (suc-+ x y)
suc-+ 2[1+ x ] 1+[2 y ] =  cong (suc ∘ 1+[2_]) (suc-+ x y)
suc-+ 1+[2 x ] 2[1+ y ] =  refl
suc-+ 1+[2 x ] 1+[2 y ] =  refl

1+≗suc : (1ᵇ +_) ≗ suc
1+≗suc = suc-+ zero

fromℕ-homo-+ : ∀ m n → fromℕ (m ℕ.+ n) ≡ fromℕ m + fromℕ n
fromℕ-homo-+ 0         _ = refl
fromℕ-homo-+ (ℕ.suc m) n = begin
  fromℕ ((ℕ.suc m) ℕ.+ n)          ≡⟨⟩
  suc (fromℕ (m ℕ.+ n))            ≡⟨ cong suc (fromℕ-homo-+ m n) ⟩
  suc (a + b)                      ≡⟨ sym (suc-+ a b) ⟩
  (suc a) + b                      ≡⟨⟩
  (fromℕ (ℕ.suc m)) + (fromℕ n)    ∎
  where open ≡-Reasoning;  a = fromℕ m;  b = fromℕ n

------------------------------------------------------------------------
-- Algebraic properties of _+_

-- Mostly proved by using the isomorphism between `ℕ` and `ℕᵇ` provided
-- by `toℕ`/`fromℕ`.

private
  module +-Monomorphism = MonoidMonomorphism toℕ-isMonoidMonomorphism-+

+-assoc : Associative _+_
+-assoc = +-Monomorphism.assoc ℕₚ.+-isMagma ℕₚ.+-assoc

+-comm : Commutative _+_
+-comm = +-Monomorphism.comm ℕₚ.+-isMagma ℕₚ.+-comm

+-identityˡ : LeftIdentity zero _+_
+-identityˡ _ = refl

+-identityʳ : RightIdentity zero _+_
+-identityʳ = +-Monomorphism.identityʳ ℕₚ.+-isMagma ℕₚ.+-identityʳ

+-identity : Identity zero _+_
+-identity = +-identityˡ , +-identityʳ

+-cancelˡ-≡ : LeftCancellative _+_
+-cancelˡ-≡ = +-Monomorphism.cancelˡ ℕₚ.+-isMagma ℕₚ.+-cancelˡ-≡

+-cancelʳ-≡ : RightCancellative _+_
+-cancelʳ-≡ = +-Monomorphism.cancelʳ ℕₚ.+-isMagma ℕₚ.+-cancelʳ-≡

------------------------------------------------------------------------
-- Structures for _+_

+-isMagma : IsMagma _+_
+-isMagma = isMagma _+_

+-isSemigroup : IsSemigroup _+_
+-isSemigroup = +-Monomorphism.isSemigroup ℕₚ.+-isSemigroup

+-isCommutativeSemigroup : IsCommutativeSemigroup _+_
+-isCommutativeSemigroup = record
  { isSemigroup = +-isSemigroup
  ; comm        = +-comm
  }

+-0-isMonoid : IsMonoid _+_ 0ᵇ
+-0-isMonoid = +-Monomorphism.isMonoid ℕₚ.+-0-isMonoid

+-0-isCommutativeMonoid : IsCommutativeMonoid _+_ 0ᵇ
+-0-isCommutativeMonoid = +-Monomorphism.isCommutativeMonoid ℕₚ.+-0-isCommutativeMonoid

------------------------------------------------------------------------
-- Bundles for _+_

+-magma : Magma 0ℓ 0ℓ
+-magma = magma _+_

+-semigroup : Semigroup 0ℓ 0ℓ
+-semigroup = record
  { isSemigroup = +-isSemigroup
  }

+-commutativeSemigroup : CommutativeSemigroup 0ℓ 0ℓ
+-commutativeSemigroup = record
  { isCommutativeSemigroup = +-isCommutativeSemigroup
  }

+-0-monoid : Monoid 0ℓ 0ℓ
+-0-monoid = record
  { ε        = zero
  ; isMonoid = +-0-isMonoid
  }

+-0-commutativeMonoid : CommutativeMonoid 0ℓ 0ℓ
+-0-commutativeMonoid = record
  { isCommutativeMonoid = +-0-isCommutativeMonoid
  }

module Bin+CSemigroup = CommSemigProp +-commutativeSemigroup

------------------------------------------------------------------------------
-- Properties of _+_ and _≤_

+-mono-≤ : _+_ Preserves₂ _≤_ ⟶ _≤_ ⟶ _≤_
+-mono-≤ {x} {x′} {y} {y′} x≤x′ y≤y′ =  begin
  x + y                 ≡⟨ sym $ cong₂ _+_ (fromℕ-toℕ x) (fromℕ-toℕ y) ⟩
  fromℕ m + fromℕ n     ≡⟨ sym (fromℕ-homo-+ m n) ⟩
  fromℕ (m ℕ.+ n)       ≤⟨ fromℕ-mono-≤ (ℕₚ.+-mono-≤ m≤m′ n≤n′) ⟩
  fromℕ (m′ ℕ.+ n′)     ≡⟨ fromℕ-homo-+ m′ n′ ⟩
  fromℕ m′ + fromℕ n′   ≡⟨ cong₂ _+_ (fromℕ-toℕ x′) (fromℕ-toℕ y′) ⟩
  x′ + y′               ∎
  where
  open ≤-Reasoning
  m    = toℕ x;             m′   = toℕ x′
  n    = toℕ y;             n′   = toℕ y′
  m≤m′ = toℕ-mono-≤ x≤x′;   n≤n′ = toℕ-mono-≤ y≤y′

+-monoˡ-≤ : ∀ x → (_+ x) Preserves _≤_ ⟶ _≤_
+-monoˡ-≤ x y≤z =  +-mono-≤ y≤z (≤-refl {x})

+-monoʳ-≤ : ∀ x → (x +_) Preserves _≤_ ⟶ _≤_
+-monoʳ-≤ x y≤z =  +-mono-≤ (≤-refl {x}) y≤z

+-mono-<-≤ : _+_ Preserves₂ _<_ ⟶ _≤_ ⟶ _<_
+-mono-<-≤ {x} {x′} {y} {y′} x<x′ y≤y′ =  begin-strict
  x + y                  ≡⟨ sym $ cong₂ _+_ (fromℕ-toℕ x) (fromℕ-toℕ y) ⟩
  fromℕ m + fromℕ n      ≡⟨ sym (fromℕ-homo-+ m n) ⟩
  fromℕ (m ℕ.+ n)        <⟨ fromℕ-mono-< (ℕₚ.+-mono-<-≤ m<m′ n≤n′) ⟩
  fromℕ (m′ ℕ.+ n′)      ≡⟨ fromℕ-homo-+ m′ n′ ⟩
  fromℕ m′ + fromℕ n′    ≡⟨ cong₂ _+_ (fromℕ-toℕ x′) (fromℕ-toℕ y′) ⟩
  x′ + y′                ∎
  where
  open ≤-Reasoning
  m    = toℕ x;             n    = toℕ y
  m′   = toℕ x′;            n′   = toℕ y′
  m<m′ = toℕ-mono-< x<x′;   n≤n′ = toℕ-mono-≤ y≤y′

+-mono-≤-< : _+_ Preserves₂ _≤_ ⟶ _<_ ⟶ _<_
+-mono-≤-< {x} {x′} {y} {y′} x≤x′ y<y′ =  subst₂ _<_ (+-comm y x) (+-comm y′ x′) y+x<y′+x′
  where
  y+x<y′+x′ =  +-mono-<-≤ y<y′ x≤x′

+-monoˡ-< : ∀ x → (_+ x) Preserves _<_ ⟶ _<_
+-monoˡ-< x y<z =  +-mono-<-≤ y<z (≤-refl {x})

+-monoʳ-< : ∀ x → (x +_) Preserves _<_ ⟶ _<_
+-monoʳ-< x y<z =  +-mono-≤-< (≤-refl {x}) y<z

x≤y+x : ∀ x y → x ≤ y + x
x≤y+x x y =  begin
  x        ≡⟨ sym (+-identityˡ x) ⟩
  0ᵇ + x   ≤⟨ +-monoˡ-≤ x (0≤x y) ⟩
  y + x    ∎
  where open ≤-Reasoning

x≤x+y : ∀ x y → x ≤ x + y
x≤x+y x y =  begin
  x        ≤⟨ x≤y+x x y ⟩
  y + x    ≡⟨ +-comm y x ⟩
  x + y    ∎
  where open ≤-Reasoning

x<x+y : ∀ x {y} → y > 0ᵇ → x < x + y
x<x+y x {y} y>0 = begin-strict
  x                             ≡⟨ sym (fromℕ-toℕ x) ⟩
  fromℕ (toℕ x)                 <⟨ fromℕ-mono-< (ℕₚ.m<m+n (toℕ x) (toℕ-mono-< y>0)) ⟩
  fromℕ (toℕ x ℕ.+ toℕ y)       ≡⟨ fromℕ-homo-+ (toℕ x) (toℕ y) ⟩
  fromℕ (toℕ x) + fromℕ (toℕ y) ≡⟨ cong₂ _+_ (fromℕ-toℕ x) (fromℕ-toℕ y) ⟩
  x + y                         ∎
  where open ≤-Reasoning

x<x+1 : ∀ x → x < x + 1ᵇ
x<x+1 x = x<x+y x 0<odd

x<1+x : ∀ x → x < 1ᵇ + x
x<1+x x rewrite +-comm 1ᵇ x = x<x+1 x

x<1⇒x≡0 : ∀ {x} → x < 1ᵇ → x ≡ zero
x<1⇒x≡0 0<odd = refl

------------------------------------------------------------------------
-- Other properties

x≢0⇒x+y≢0 : ∀ {x} (y : ℕᵇ) → x ≢ zero → x + y ≢ zero
x≢0⇒x+y≢0 {2[1+ _ ]} zero _   =  λ()
x≢0⇒x+y≢0 {zero}     _    0≢0 =  contradiction refl 0≢0

------------------------------------------------------------------------
-- Properties of _*_
------------------------------------------------------------------------

------------------------------------------------------------------------
-- Raw bundles for _*_

*-rawMagma : RawMagma 0ℓ 0ℓ
*-rawMagma = record
  { _≈_ = _≡_
  ; _∙_ = _*_
  }

*-1-rawMonoid : RawMonoid 0ℓ 0ℓ
*-1-rawMonoid = record
  { _≈_ = _≡_
  ; _∙_ = _*_
  ; ε   = 1ᵇ
  }

------------------------------------------------------------------------
-- toℕ/fromℕ are homomorphisms for _*_

private  2*ₙ2*ₙ =  (2 ℕ.*_) ∘ (2 ℕ.*_)

toℕ-homo-* : ∀ x y → toℕ (x * y) ≡ toℕ x ℕ.* toℕ y
toℕ-homo-* x y =  aux x y (size x ℕ.+ size y) ℕₚ.≤-refl
  where
  aux : (x y : ℕᵇ) → (cnt : ℕ) → (size x ℕ.+ size y ℕ.≤ cnt) →  toℕ (x * y) ≡ toℕ x ℕ.* toℕ y
  aux zero     _        _ _ = refl
  aux 2[1+ x ] zero     _ _ = sym (ℕₚ.*-zeroʳ (toℕ x ℕ.+ (ℕ.suc (toℕ x ℕ.+ 0))))
  aux 1+[2 x ] zero     _ _ = sym (ℕₚ.*-zeroʳ (toℕ x ℕ.+ (toℕ x ℕ.+ 0)))
  aux 2[1+ x ] 2[1+ y ] (ℕ.suc cnt) (s≤s |x|+1+|y|≤cnt) = begin
    toℕ (2[1+ x ] * 2[1+ y ])                ≡⟨⟩
    toℕ (double 2[1+ (x + (y + xy)) ])       ≡⟨ toℕ-double 2[1+ (x + (y + xy)) ] ⟩
    2 ℕ.* (toℕ 2[1+ (x + (y + xy)) ])        ≡⟨⟩
    2*ₙ2*ₙ (ℕ.suc (toℕ (x + (y + xy))))      ≡⟨ cong (2*ₙ2*ₙ ∘ ℕ.suc) (toℕ-homo-+ x (y + xy)) ⟩
    2*ₙ2*ₙ (ℕ.suc (m ℕ.+ (toℕ (y + xy))))    ≡⟨ cong (2*ₙ2*ₙ ∘ ℕ.suc ∘ (m ℕ.+_)) (toℕ-homo-+ y xy) ⟩
    2*ₙ2*ₙ (ℕ.suc (m ℕ.+ (n ℕ.+ toℕ xy)))    ≡⟨ cong (2*ₙ2*ₙ ∘ ℕ.suc ∘ (m ℕ.+_) ∘ (n ℕ.+_))
                                                  (aux x y cnt |x|+|y|≤cnt) ⟩
    2*ₙ2*ₙ (ℕ.suc (m ℕ.+ (n ℕ.+ (m ℕ.* n)))) ≡⟨ solve 2 (λ m n → con 2 :* (con 2 :* (con 1 :+ (m :+ (n :+ m :* n)))) :=
                                                  (con 2 :* (con 1 :+ m)) :* (con 2 :* (con 1 :+ n)))
                                                  refl m n ⟩
    (2 ℕ.* (1 ℕ.+ m)) ℕ.* (2 ℕ.* (1 ℕ.+ n))  ≡⟨⟩
    toℕ 2[1+ x ] ℕ.* toℕ 2[1+ y ]            ∎
    where
    open ≡-Reasoning;  m = toℕ x;  n = toℕ y;  xy = x * y

    |x|+|y|≤cnt = ℕₚ.≤-trans (ℕₚ.+-monoʳ-≤ (size x) (ℕₚ.n≤1+n (size y))) |x|+1+|y|≤cnt

  aux 2[1+ x ] 1+[2 y ] (ℕ.suc cnt) (s≤s |x|+1+|y|≤cnt) = begin
    toℕ (2[1+ x ] * 1+[2 y ])                  ≡⟨⟩
    toℕ (2[1+ (x + y * 2[1+ x ]) ])            ≡⟨⟩
    2 ℕ.* (ℕ.suc (toℕ (x + y * 2[1+ x ])))     ≡⟨ cong ((2 ℕ.*_) ∘ ℕ.suc) (toℕ-homo-+ x _) ⟩
    2 ℕ.* (ℕ.suc (m ℕ.+ (toℕ (y * 2[1+ x ])))) ≡⟨ cong ((2 ℕ.*_) ∘ ℕ.suc ∘ (m ℕ.+_))
                                                    (aux y 2[1+ x ] cnt |y|+1+|x|≤cnt) ⟩
    2 ℕ.* (1+m ℕ.+ (n ℕ.* (toℕ 2[1+ x ])))     ≡⟨⟩
    2 ℕ.* (1+m ℕ.+ (n ℕ.* 2[1+m]))             ≡⟨ solve 2 (λ m n →
                                                    con 2 :* ((con 1 :+ m) :+ (n :* (con 2 :* (con 1 :+ m)))) :=
                                                    (con 2 :* (con 1 :+ m)) :* (con 1 :+ con 2 :* n))
                                                    refl m n ⟩
    2[1+m] ℕ.* (ℕ.suc (2 ℕ.* n))               ≡⟨⟩
    toℕ 2[1+ x ] ℕ.* toℕ 1+[2 y ]              ∎
    where
    open ≡-Reasoning;   m = toℕ x;  n = toℕ y;  1+m = ℕ.suc m;  2[1+m] = 2 ℕ.* (ℕ.suc m)

    eq : size x ℕ.+ (ℕ.suc (size y)) ≡ size y ℕ.+ (ℕ.suc (size x))
    eq = ℕ-+-semigroupProperties.x∙yz≈z∙yx (size x) 1 _

    |y|+1+|x|≤cnt =  subst (ℕ._≤ cnt) eq |x|+1+|y|≤cnt

  aux 1+[2 x ] 2[1+ y ] (ℕ.suc cnt) (s≤s |x|+1+|y|≤cnt) = begin
    toℕ (1+[2 x ] * 2[1+ y ])                  ≡⟨⟩
    toℕ 2[1+ (y + x * 2[1+ y ]) ]              ≡⟨⟩
    2 ℕ.* (ℕ.suc (toℕ (y + x * 2[1+ y ])))     ≡⟨ cong ((2 ℕ.*_) ∘ ℕ.suc)
                                                    (toℕ-homo-+ y (x * 2[1+ y ])) ⟩
    2 ℕ.* (ℕ.suc (n ℕ.+ (toℕ (x * 2[1+ y ])))) ≡⟨ cong ((2 ℕ.*_) ∘ ℕ.suc ∘ (n ℕ.+_))
                                                    (aux x 2[1+ y ] cnt |x|+1+|y|≤cnt) ⟩
    2 ℕ.* (1+n ℕ.+ (m ℕ.* toℕ 2[1+ y ]))       ≡⟨⟩
    2 ℕ.* (1+n ℕ.+ (m ℕ.* 2[1+n]))             ≡⟨ solve 2 (λ m n →
                                                    con 2 :* ((con 1 :+ n) :+ (m :* (con 2 :* (con 1 :+ n)))) :=
                                                    (con 1 :+ (con 2 :* m)) :* (con 2 :* (con 1 :+ n)))
                                                    refl m n ⟩
    (ℕ.suc 2m) ℕ.* 2[1+n]                      ≡⟨⟩
    toℕ 1+[2 x ] ℕ.* toℕ 2[1+ y ]              ∎
    where
    open ≡-Reasoning
    m  = toℕ x;     n      = toℕ y;            1+n = ℕ.suc n
    2m = 2 ℕ.* m;   2[1+n] = 2 ℕ.* (ℕ.suc n)

  aux 1+[2 x ] 1+[2 y ] (ℕ.suc cnt) (s≤s |x|+1+|y|≤cnt) = begin
    toℕ (1+[2 x ] * 1+[2 y ])               ≡⟨⟩
    toℕ 1+[2 (x + y * 1+2x) ]               ≡⟨⟩
    ℕ.suc (2 ℕ.* (toℕ (x + y * 1+2x)))      ≡⟨ cong (ℕ.suc ∘ (2 ℕ.*_)) (toℕ-homo-+ x (y * 1+2x)) ⟩
    ℕ.suc (2 ℕ.* (m ℕ.+ (toℕ (y * 1+2x))))  ≡⟨ cong (ℕ.suc ∘ (2 ℕ.*_) ∘ (m ℕ.+_))
                                                 (aux y 1+2x cnt |y|+1+|x|≤cnt) ⟩
    ℕ.suc (2 ℕ.* (m ℕ.+ (n ℕ.* [1+2x]′)))   ≡⟨ cong ℕ.suc $ ℕₚ.*-distribˡ-+ 2 m (n ℕ.* [1+2x]′) ⟩
    ℕ.suc (2m ℕ.+ (2 ℕ.* (n ℕ.* [1+2x]′)))  ≡⟨ cong (ℕ.suc ∘ (2m ℕ.+_)) (sym (ℕₚ.*-assoc 2 n _)) ⟩
    (ℕ.suc 2m) ℕ.+ 2n ℕ.* [1+2x]′           ≡⟨⟩
    [1+2x]′ ℕ.+ 2n ℕ.* [1+2x]′              ≡⟨ cong (ℕ._+ (2n ℕ.* [1+2x]′)) $
                                                    sym (ℕₚ.*-identityˡ [1+2x]′) ⟩
    1 ℕ.* [1+2x]′ ℕ.+ 2n ℕ.* [1+2x]′        ≡⟨ sym (ℕₚ.*-distribʳ-+ [1+2x]′ 1 2n) ⟩
    (ℕ.suc 2n) ℕ.* [1+2x]′                  ≡⟨ ℕₚ.*-comm (ℕ.suc 2n) [1+2x]′ ⟩
    toℕ 1+[2 x ] ℕ.* toℕ 1+[2 y ]           ∎
    where
    open ≡-Reasoning
    m    = toℕ x;      n       = toℕ y;     2m = 2 ℕ.* m;    2n = 2 ℕ.* n
    1+2x = 1+[2 x ];   [1+2x]′ = toℕ 1+2x

    eq : size x ℕ.+ (ℕ.suc (size y)) ≡ size y ℕ.+ (ℕ.suc (size x))
    eq = ℕ-+-semigroupProperties.x∙yz≈z∙yx (size x) 1 _

    |y|+1+|x|≤cnt = subst (ℕ._≤ cnt) eq |x|+1+|y|≤cnt


toℕ-isMagmaHomomorphism-* : IsMagmaHomomorphism *-rawMagma ℕₚ.*-rawMagma toℕ
toℕ-isMagmaHomomorphism-* = record
  { isRelHomomorphism = toℕ-isRelHomomorphism
  ; homo              = toℕ-homo-*
  }

toℕ-isMonoidHomomorphism-* : IsMonoidHomomorphism *-1-rawMonoid ℕₚ.*-1-rawMonoid toℕ
toℕ-isMonoidHomomorphism-* = record
  { isMagmaHomomorphism = toℕ-isMagmaHomomorphism-*
  ; ε-homo              = refl
  }

toℕ-isMonoidMonomorphism-* : IsMonoidMonomorphism *-1-rawMonoid ℕₚ.*-1-rawMonoid toℕ
toℕ-isMonoidMonomorphism-* = record
  { isMonoidHomomorphism = toℕ-isMonoidHomomorphism-*
  ; injective            = toℕ-injective
  }

fromℕ-homo-* : ∀ m n → fromℕ (m ℕ.* n) ≡ fromℕ m * fromℕ n
fromℕ-homo-* m n = begin
  fromℕ (m ℕ.* n)           ≡⟨ cong fromℕ (cong₂ ℕ._*_ m≡aN n≡bN) ⟩
  fromℕ (toℕ a ℕ.* toℕ b)   ≡⟨ cong fromℕ (sym (toℕ-homo-* a b)) ⟩
  fromℕ (toℕ (a * b))       ≡⟨ fromℕ-toℕ (a * b) ⟩
  a * b                     ∎
  where
  open ≡-Reasoning
  a    = fromℕ m;             b    = fromℕ n
  m≡aN = sym (toℕ-fromℕ m);   n≡bN = sym (toℕ-fromℕ n)

private
  module *-Monomorphism = MonoidMonomorphism toℕ-isMonoidMonomorphism-*

------------------------------------------------------------------------
-- Algebraic properties of _*_

-- Mostly proved by using the isomorphism between `ℕ` and `ℕᵇ` provided
-- by `toℕ`/`fromℕ`.

*-assoc : Associative _*_
*-assoc = *-Monomorphism.assoc ℕₚ.*-isMagma ℕₚ.*-assoc

*-comm : Commutative _*_
*-comm = *-Monomorphism.comm ℕₚ.*-isMagma ℕₚ.*-comm

*-identityˡ : LeftIdentity 1ᵇ _*_
*-identityˡ = *-Monomorphism.identityˡ ℕₚ.*-isMagma ℕₚ.*-identityˡ

*-identityʳ : RightIdentity 1ᵇ _*_
*-identityʳ x =  trans (*-comm x 1ᵇ) (*-identityˡ x)

*-identity : Identity 1ᵇ _*_
*-identity = (*-identityˡ , *-identityʳ)

*-zeroˡ : LeftZero zero _*_
*-zeroˡ _ = refl

*-zeroʳ : RightZero zero _*_
*-zeroʳ zero     = refl
*-zeroʳ 2[1+ _ ] = refl
*-zeroʳ 1+[2 _ ] = refl

*-zero : Zero zero _*_
*-zero = *-zeroˡ , *-zeroʳ

*-distribˡ-+ : _*_ DistributesOverˡ _+_
*-distribˡ-+ a b c = begin
  a * (b + c)                          ≡⟨ sym (fromℕ-toℕ (a * (b + c))) ⟩
  fromℕ (toℕ (a * (b + c)))            ≡⟨ cong fromℕ (toℕ-homo-* a (b + c)) ⟩
  fromℕ (k ℕ.* (toℕ (b + c)))          ≡⟨ cong (fromℕ ∘ (k ℕ.*_)) (toℕ-homo-+ b c) ⟩
  fromℕ (k ℕ.* (m ℕ.+ n))              ≡⟨ cong fromℕ (ℕₚ.*-distribˡ-+ k m n) ⟩
  fromℕ (k ℕ.* m ℕ.+ k ℕ.* n)          ≡⟨ cong fromℕ $ sym $
                                            cong₂ ℕ._+_ (toℕ-homo-* a b) (toℕ-homo-* a c) ⟩
  fromℕ (toℕ (a * b) ℕ.+ toℕ (a * c))  ≡⟨ cong fromℕ (sym (toℕ-homo-+ (a * b) (a * c))) ⟩
  fromℕ (toℕ (a * b + a * c))          ≡⟨ fromℕ-toℕ (a * b + a * c) ⟩
  a * b + a * c                        ∎
  where open ≡-Reasoning;  k = toℕ a;  m = toℕ b;  n = toℕ c

*-distribʳ-+ : _*_ DistributesOverʳ _+_
*-distribʳ-+ = comm+distrˡ⇒distrʳ *-comm *-distribˡ-+

*-distrib-+ : _*_ DistributesOver _+_
*-distrib-+ = *-distribˡ-+ , *-distribʳ-+

------------------------------------------------------------------------
-- Structures

*-isMagma : IsMagma _*_
*-isMagma = isMagma _*_

*-isSemigroup : IsSemigroup _*_
*-isSemigroup = *-Monomorphism.isSemigroup ℕₚ.*-isSemigroup

*-1-isMonoid : IsMonoid _*_ 1ᵇ
*-1-isMonoid = *-Monomorphism.isMonoid ℕₚ.*-1-isMonoid

*-1-isCommutativeMonoid : IsCommutativeMonoid _*_ 1ᵇ
*-1-isCommutativeMonoid = *-Monomorphism.isCommutativeMonoid ℕₚ.*-1-isCommutativeMonoid

*-+-isSemiringWithoutAnnihilatingZero : IsSemiringWithoutAnnihilatingZero _+_ _*_ zero 1ᵇ
*-+-isSemiringWithoutAnnihilatingZero = record
  { +-isCommutativeMonoid = +-0-isCommutativeMonoid
  ; *-isMonoid            = *-1-isMonoid
  ; distrib               = *-distrib-+
  }

*-+-isSemiring : IsSemiring _+_ _*_ zero 1ᵇ
*-+-isSemiring = record
  { isSemiringWithoutAnnihilatingZero = *-+-isSemiringWithoutAnnihilatingZero
  ; zero                              = *-zero
  }

*-+-isCommutativeSemiring : IsCommutativeSemiring _+_ _*_ zero 1ᵇ
*-+-isCommutativeSemiring = record
  { isSemiring = *-+-isSemiring
  ; *-comm     = *-comm
  }

------------------------------------------------------------------------
-- Bundles

*-magma : Magma 0ℓ 0ℓ
*-magma = record
  { isMagma = *-isMagma
  }

*-semigroup : Semigroup 0ℓ 0ℓ
*-semigroup = record
  { isSemigroup = *-isSemigroup
  }

*-1-monoid : Monoid 0ℓ 0ℓ
*-1-monoid = record
  { isMonoid = *-1-isMonoid
  }

*-1-commutativeMonoid : CommutativeMonoid 0ℓ 0ℓ
*-1-commutativeMonoid = record
  { isCommutativeMonoid = *-1-isCommutativeMonoid
  }

*-+-semiring : Semiring 0ℓ 0ℓ
*-+-semiring = record
  { isSemiring = *-+-isSemiring
  }

*-+-commutativeSemiring : CommutativeSemiring 0ℓ 0ℓ
*-+-commutativeSemiring = record
  { isCommutativeSemiring = *-+-isCommutativeSemiring
  }

------------------------------------------------------------------------
-- Properties of _*_ and _≤_ & _<_

*-mono-≤ : _*_ Preserves₂ _≤_ ⟶ _≤_ ⟶ _≤_
*-mono-≤ {x} {u} {y} {v} x≤u y≤v = toℕ-cancel-≤ (begin
  toℕ (x * y)      ≡⟨ toℕ-homo-* x y ⟩
  toℕ x ℕ.* toℕ y  ≤⟨ ℕₚ.*-mono-≤ (toℕ-mono-≤ x≤u) (toℕ-mono-≤ y≤v) ⟩
  toℕ u ℕ.* toℕ v  ≡⟨ sym (toℕ-homo-* u v) ⟩
  toℕ (u * v)      ∎)
  where open ℕₚ.≤-Reasoning

*-monoʳ-≤ : ∀ x → (x *_) Preserves _≤_ ⟶ _≤_
*-monoʳ-≤ x y≤y′ = *-mono-≤ (≤-refl {x}) y≤y′

*-monoˡ-≤ : ∀ x → (_* x) Preserves _≤_ ⟶ _≤_
*-monoˡ-≤ x y≤y′ = *-mono-≤ y≤y′ (≤-refl {x})

*-mono-< : _*_ Preserves₂ _<_ ⟶ _<_ ⟶ _<_
*-mono-< {x} {u} {y} {v} x<u y<v = toℕ-cancel-< (begin-strict
  toℕ (x * y)      ≡⟨ toℕ-homo-* x y ⟩
  toℕ x ℕ.* toℕ y  <⟨ ℕₚ.*-mono-< (toℕ-mono-< x<u) (toℕ-mono-< y<v) ⟩
  toℕ u ℕ.* toℕ v  ≡⟨ sym (toℕ-homo-* u v) ⟩
  toℕ (u * v)      ∎)
  where open ℕₚ.≤-Reasoning

*-monoʳ-< : ∀ x → ((1ᵇ + x) *_) Preserves _<_ ⟶ _<_
*-monoʳ-< x {y} {z} y<z = begin-strict
  (1ᵇ + x) * y    ≡⟨ *-distribʳ-+ y 1ᵇ x ⟩
  1ᵇ * y + x * y  ≡⟨ cong (_+ x * y) (*-identityˡ y) ⟩
  y      + x * y  <⟨ +-mono-<-≤ y<z (*-monoʳ-≤ x (<⇒≤ y<z)) ⟩
  z      + x * z  ≡⟨ cong (_+ x * z) (sym (*-identityˡ z)) ⟩
  1ᵇ * z + x * z  ≡⟨ sym (*-distribʳ-+ z 1ᵇ x) ⟩
  (1ᵇ + x) * z    ∎
  where open ≤-Reasoning

*-monoˡ-< : ∀ x → (_* (1ᵇ + x)) Preserves _<_ ⟶ _<_
*-monoˡ-< x {y} {z} y<z = begin-strict
  y * (1ᵇ + x)   ≡⟨ *-comm y (1ᵇ + x) ⟩
  (1ᵇ + x) * y   <⟨ *-monoʳ-< x y<z ⟩
  (1ᵇ + x) * z   ≡⟨ *-comm (1ᵇ + x) z ⟩
  z * (1ᵇ + x)   ∎
  where open ≤-Reasoning

------------------------------------------------------------------------
-- Other properties of _*_

x*y≡0⇒x≡0∨y≡0 : ∀ x {y} → x * y ≡ zero → x ≡ zero ⊎ y ≡ zero
x*y≡0⇒x≡0∨y≡0 zero {_}    _ =  inj₁ refl
x*y≡0⇒x≡0∨y≡0 _    {zero} _ =  inj₂ refl

x≢0∧y≢0⇒x*y≢0 : ∀ {x y} → x ≢ zero → y ≢ zero → x * y ≢ zero
x≢0∧y≢0⇒x*y≢0 {x} {_} x≢0 y≢0 xy≡0  with x*y≡0⇒x≡0∨y≡0 x xy≡0
... | inj₁ x≡0 =  x≢0 x≡0
... | inj₂ y≡0 =  y≢0 y≡0

2*x≡x+x : ∀ x → 2ᵇ * x ≡ x + x
2*x≡x+x x = begin
  2ᵇ * x            ≡⟨⟩
  (1ᵇ + 1ᵇ) * x     ≡⟨ *-distribʳ-+ x 1ᵇ 1ᵇ ⟩
  1ᵇ * x + 1ᵇ * x   ≡⟨ cong₂ _+_ (*-identityˡ x) (*-identityˡ x) ⟩
  x + x             ∎
  where open ≡-Reasoning

1+-* : ∀ x y → (1ᵇ + x) * y ≡ y + x * y
1+-* x y = begin
  (1ᵇ + x) * y     ≡⟨ *-distribʳ-+ y 1ᵇ x ⟩
  1ᵇ * y + x * y   ≡⟨ cong (_+ x * y) (*-identityˡ y) ⟩
  y + x * y        ∎
  where open ≡-Reasoning

*-1+ : ∀ x y → y * (1ᵇ + x) ≡ y + y * x
*-1+ x y = begin
  y * (1ᵇ + x)     ≡⟨ *-distribˡ-+ y 1ᵇ x ⟩
  y * 1ᵇ + y * x   ≡⟨ cong (_+ y * x) (*-identityʳ y) ⟩
  y + y * x        ∎
  where open ≡-Reasoning

------------------------------------------------------------------------
-- Properties of double
------------------------------------------------------------------------

double[x]≡0⇒x≡0 : ∀ {x} → double x ≡ zero → x ≡ zero
double[x]≡0⇒x≡0 {zero} _ = refl

x≡0⇒double[x]≡0 : ∀ {x} → x ≡ 0ᵇ → double x ≡ 0ᵇ
x≡0⇒double[x]≡0 = cong double

x≢0⇒double[x]≢0 : ∀ {x} → x ≢ zero → double x ≢ zero
x≢0⇒double[x]≢0 x≢0 = x≢0 ∘ double[x]≡0⇒x≡0

double≢1 : ∀ {x} → double x ≢ 1ᵇ
double≢1 {zero} ()

double≗2* : double ≗ 2ᵇ *_
double≗2* x =  toℕ-injective $ begin
  toℕ (double x)  ≡⟨ toℕ-double x ⟩
  2 ℕ.* (toℕ x)   ≡⟨ sym (toℕ-homo-* 2ᵇ x) ⟩
  toℕ (2ᵇ * x)    ∎
  where open ≡-Reasoning

double-*-assoc : ∀ x y → (double x) * y ≡ double (x * y)
double-*-assoc x y = begin
  (double x) * y     ≡⟨ cong (_* y) (double≗2* x) ⟩
  (2ᵇ * x) * y       ≡⟨ *-assoc 2ᵇ x y ⟩
  2ᵇ * (x * y)       ≡⟨ sym (double≗2* (x * y)) ⟩
  double (x * y)     ∎
  where open ≡-Reasoning

double[x]≡x+x : ∀ x → double x ≡ x + x
double[x]≡x+x x =  trans (double≗2* x) (2*x≡x+x x)

double-distrib-+ : ∀ x y → double (x + y) ≡ double x + double y
double-distrib-+ x y = begin
  double (x + y)         ≡⟨ double≗2* (x + y) ⟩
  2ᵇ * (x + y)           ≡⟨ *-distribˡ-+ 2ᵇ x y ⟩
  (2ᵇ * x) + (2ᵇ * y)    ≡⟨ sym (cong₂ _+_ (double≗2* x) (double≗2* y)) ⟩
  double x + double y    ∎
  where open ≡-Reasoning

double-mono-≤ : double Preserves _≤_ ⟶ _≤_
double-mono-≤ {x} {y} x≤y =  begin
  double x   ≡⟨ double≗2* x ⟩
  2ᵇ * x     ≤⟨ *-monoʳ-≤ 2ᵇ x≤y ⟩
  2ᵇ * y     ≡⟨ sym (double≗2* y) ⟩
  double y   ∎
  where open ≤-Reasoning

double-mono-< : double Preserves _<_ ⟶ _<_
double-mono-< {x} {y} x<y =  begin-strict
  double x   ≡⟨ double≗2* x ⟩
  2ᵇ * x     <⟨ *-monoʳ-< 1ᵇ x<y ⟩
  2ᵇ * y     ≡⟨ sym (double≗2* y) ⟩
  double y   ∎
  where open ≤-Reasoning

double-cancel-≤ : ∀ {x y} → double x ≤ double y → x ≤ y
double-cancel-≤ {x} {y} 2x≤2y  with <-cmp x y
... | tri< x<y _   _   =  <⇒≤ x<y
... | tri≈ _   x≡y _   =  ≤-reflexive x≡y
... | tri> _   _   x>y =  contradiction 2x≤2y (<⇒≱ (double-mono-< x>y))

double-cancel-< : ∀ {x y} → double x < double y → x < y
double-cancel-< {x} {y} 2x<2y  with <-cmp x y
... | tri< x<y _    _   =  x<y
... | tri≈ _   refl _   =  contradiction 2x<2y (<-irrefl refl)
... | tri> _   _    x>y =  contradiction (double-mono-< x>y) (<⇒≯ 2x<2y)

x<double[x] : ∀ x → x ≢ zero → x < double x
x<double[x] x x≢0 = begin-strict
  x                 <⟨ x<x+y x (x≢0⇒x>0 x≢0) ⟩
  x + x             ≡⟨ sym (double[x]≡x+x x) ⟩
  double x          ∎
  where open ≤-Reasoning

x≤double[x] : ∀ x → x ≤ double x
x≤double[x] x =  begin
  x         ≤⟨ x≤x+y x x ⟩
  x + x     ≡⟨ sym (double[x]≡x+x x) ⟩
  double x  ∎
  where open ≤-Reasoning

double-suc : ∀ x → double (suc x) ≡ 2ᵇ + double x
double-suc x = begin
  double (suc x)   ≡⟨ cong double (suc≗1+ x) ⟩
  double (1ᵇ + x)  ≡⟨ double-distrib-+ 1ᵇ x ⟩
  2ᵇ + double x    ∎
  where open ≡-Reasoning



------------------------------------------------------------------------
-- Properties of suc
------------------------------------------------------------------------

2[1+_]-double-suc : 2[1+_] ≗ double ∘ suc
2[1+_]-double-suc zero     = refl
2[1+_]-double-suc 2[1+ x ] = cong 2[1+_] (2[1+_]-double-suc x)
2[1+_]-double-suc 1+[2 x ] = refl

1+[2_]-suc-double : 1+[2_] ≗ suc ∘ double
1+[2_]-suc-double zero     = refl
1+[2_]-suc-double 2[1+ x ] = refl
1+[2_]-suc-double 1+[2 x ] = begin
  1+[2 1+[2 x ] ]         ≡⟨ cong 1+[2_] (1+[2_]-suc-double x) ⟩
  1+[2 (suc 2x) ]         ≡⟨⟩
  suc 2[1+ 2x ]           ≡⟨ cong suc (2[1+_]-double-suc 2x) ⟩
  suc (double (suc 2x))   ≡⟨ cong (suc ∘ double) (sym (1+[2_]-suc-double x)) ⟩
  suc (double 1+[2 x ])   ∎
  where open ≡-Reasoning;  2x = double x

suc≢0 : ∀ {x} → suc x ≢ zero
suc≢0 {zero}     ()
suc≢0 {2[1+ _ ]} ()
suc≢0 {1+[2 _ ]} ()

x+suc[y]≡suc[x]+y : ∀ x y → x + suc y ≡ suc x + y
x+suc[y]≡suc[x]+y x y = begin
  x + suc y     ≡⟨ +-comm x _ ⟩
  suc y + x     ≡⟨ suc-+ y x ⟩
  suc (y + x)   ≡⟨ cong suc (+-comm y x) ⟩
  suc (x + y)   ≡⟨ sym (suc-+ x y) ⟩
  suc x + y     ∎
  where open ≡-Reasoning

0<suc : ∀ x → zero < suc x
0<suc x =  x≢0⇒x>0 (suc≢0 {x})

x<suc[x] : ∀ x → x < suc x
x<suc[x] x = begin-strict
  x        <⟨ x<1+x x ⟩
  1ᵇ + x   ≡⟨ sym (suc≗1+ x) ⟩
  suc x    ∎
  where open ≤-Reasoning

x≤suc[x] : ∀ x → x ≤ suc x
x≤suc[x] x = <⇒≤ (x<suc[x] x)

x≢suc[x] : ∀ x → x ≢ suc x
x≢suc[x] x = <⇒≢ (x<suc[x] x)

suc-mono-≤ : suc Preserves _≤_ ⟶ _≤_
suc-mono-≤ {x} {y} x≤y =  begin
  suc x     ≡⟨ suc≗1+ x ⟩
  1ᵇ + x    ≤⟨ +-monoʳ-≤ 1ᵇ x≤y ⟩
  1ᵇ + y    ≡⟨ sym (suc≗1+ y) ⟩
  suc y     ∎
  where open ≤-Reasoning

suc[x]≤y⇒x<y : ∀ {x y} → suc x ≤ y → x < y
suc[x]≤y⇒x<y {x} (inj₁ sx<y) = <-trans (x<suc[x] x) sx<y
suc[x]≤y⇒x<y {x} (inj₂ refl) = x<suc[x] x

x<y⇒suc[x]≤y : ∀ {x y} → x < y → suc x ≤ y
x<y⇒suc[x]≤y {x} {y} x<y = begin
  suc x                  ≡⟨ sym (fromℕ-toℕ (suc x)) ⟩
  fromℕ (toℕ (suc x))    ≡⟨ cong fromℕ (toℕ-suc x) ⟩
  fromℕ (ℕ.suc (toℕ x))  ≤⟨ fromℕ-mono-≤ (toℕ-mono-< x<y) ⟩
  fromℕ (toℕ y)          ≡⟨ fromℕ-toℕ y ⟩
  y                      ∎
  where open ≤-Reasoning

suc-* : ∀ x y → suc x * y ≡ y + x * y
suc-* x y = begin
  suc x * y     ≡⟨ cong (_* y) (suc≗1+ x) ⟩
  (1ᵇ + x) * y  ≡⟨ 1+-* x y ⟩
  y + x * y     ∎
  where open ≡-Reasoning

*-suc : ∀ x y → x * suc y ≡ x + x * y
*-suc x y = begin
  x * suc y     ≡⟨ cong (x *_) (suc≗1+ y) ⟩
  x * (1ᵇ + y)  ≡⟨ *-1+ y x ⟩
  x + x * y     ∎
  where open ≡-Reasoning

x≤suc[y]*x : ∀ x y → x ≤ (suc y) * x
x≤suc[y]*x x y = begin
  x             ≤⟨ x≤x+y x (y * x) ⟩
  x + y * x     ≡⟨ sym (suc-* y x) ⟩
  (suc y) * x   ∎
  where open ≤-Reasoning

suc[x]≤double[x] : ∀ x → x ≢ zero → suc x ≤ double x
suc[x]≤double[x] x =  x<y⇒suc[x]≤y {x} {double x} ∘ x<double[x] x

suc[x]<2[1+x] : ∀ x → suc x < 2[1+ x ]
suc[x]<2[1+x] x =  begin-strict
  suc x           <⟨ x<double[x] (suc x) suc≢0  ⟩
  double (suc x)  ≡⟨ sym (2[1+_]-double-suc x) ⟩
  2[1+ x ]        ∎
  where open ≤-Reasoning

double[x]<1+[2x] : ∀ x → double x < 1+[2 x ]
double[x]<1+[2x] x = begin-strict
  double x         <⟨ x<suc[x] (double x) ⟩
  suc (double x)   ≡⟨ sym (1+[2_]-suc-double x) ⟩
  1+[2 x ]         ∎
  where open ≤-Reasoning

------------------------------------------------------------------------
-- Properties of pred
------------------------------------------------------------------------

pred-suc : pred ∘ suc ≗ id
pred-suc zero     =  refl
pred-suc 2[1+ x ] =  sym (2[1+_]-double-suc x)
pred-suc 1+[2 x ] =  refl

suc-pred : ∀ {x} → x ≢ zero → suc (pred x) ≡ x
suc-pred {zero}     0≢0 =  contradiction refl 0≢0
suc-pred {2[1+ _ ]} _   =  refl
suc-pred {1+[2 x ]} _   =  sym (1+[2_]-suc-double x)

pred-mono-≤ : pred Preserves _≤_ ⟶ _≤_
pred-mono-≤ {x} {y} x≤y = begin
  pred x             ≡⟨ cong pred (sym (fromℕ-toℕ x)) ⟩
  pred (fromℕ m)     ≡⟨ sym (fromℕ-pred m) ⟩
  fromℕ (ℕ.pred m)   ≤⟨ fromℕ-mono-≤ (ℕₚ.pred-mono (toℕ-mono-≤ x≤y)) ⟩
  fromℕ (ℕ.pred n)   ≡⟨ fromℕ-pred n ⟩
  pred (fromℕ n)     ≡⟨ cong pred (fromℕ-toℕ y) ⟩
  pred y             ∎
  where
  open ≤-Reasoning;  m = toℕ x;  n = toℕ y

pred[x]<x : ∀ {x} → x ≢ zero → pred x < x
pred[x]<x {x} x≢0 = begin-strict
  pred x       <⟨ x<suc[x] (pred x) ⟩
  suc (pred x) ≡⟨ suc-pred x≢0 ⟩
  x            ∎
  where open ≤-Reasoning

pred[x]+y≡x+pred[y] : ∀ {x y} → x ≢ 0ᵇ → y ≢ 0ᵇ → (pred x) + y ≡ x + pred y
pred[x]+y≡x+pred[y] {x} {y} x≢0 y≢0 = begin
  px + y           ≡⟨ cong (px +_) (sym (suc-pred y≢0)) ⟩
  px + suc py      ≡⟨ cong (px +_) (suc≗1+ py) ⟩
  px + (1ᵇ + py)   ≡⟨ Bin+CSemigroup.x∙yz≈yx∙z px 1ᵇ py ⟩
  (1ᵇ + px) + py   ≡⟨ cong (_+ py) (sym (suc≗1+ px)) ⟩
  (suc px) + py    ≡⟨ cong (_+ py) (suc-pred x≢0) ⟩
  x + py           ∎
  where open ≡-Reasoning;  px = pred x;  py = pred y


------------------------------------------------------------------------
-- Properties of size
------------------------------------------------------------------------

|x|≡0⇒x≡0 : ∀ {x} → size x ≡ 0 → x ≡ 0ᵇ
|x|≡0⇒x≡0 {zero} refl =  refl
