------------------------------------------------------------------------
-- The Agda standard library
--
-- Properties of the heterogeneous suffix relation
------------------------------------------------------------------------

{-# OPTIONS --without-K --safe #-}

module Data.List.Relation.Binary.Suffix.Heterogeneous.Properties where

open import Data.Bool.Base using (true; false)
open import Data.List.Base as List
  using (List; []; _∷_; _++_; length; filter; replicate; reverse; reverseAcc)
open import Data.List.Relation.Binary.Pointwise as Pw
  using (Pointwise; []; _∷_; Pointwise-length)
open import Data.List.Relation.Binary.Suffix.Heterogeneous as Suffix
  using (Suffix; here; there; tail)
open import Data.List.Relation.Binary.Prefix.Heterogeneous as Prefix
  using (Prefix)
open import Data.Nat.Base
open import Data.Nat.Properties
open import Function using (_$_; flip)
open import Relation.Nullary using (Dec; does; ¬_)
import Relation.Nullary.Decidable as Dec
open import Relation.Unary as U using (Pred)
open import Relation.Nullary.Negation using (contradiction)
open import Relation.Binary as B
  using (REL; Rel; Trans; Antisym; Irrelevant; _⇒_)
open import Relation.Binary.PropositionalEquality as P
  using (_≡_; _≢_; refl; sym; subst; subst₂)

import Data.List.Properties as Listₚ
import Data.List.Relation.Binary.Prefix.Heterogeneous.Properties as Prefixₚ

------------------------------------------------------------------------
-- Suffix and Prefix are linked via reverse

module _ {a b r} {A : Set a} {B : Set b} {R : REL A B r} where

  fromPrefix : ∀ {as bs} → Prefix R as bs →
               Suffix R (reverse as) (reverse bs)
  fromPrefix {as} {bs} p with Prefix.toView p
  ... | Prefix._++_ {cs} rs ds =
    subst (Suffix R (reverse as))
      (sym (Listₚ.reverse-++-commute cs ds))
      (Suffix.fromView (reverse ds Suffix.++ Pw.reverse⁺ rs))

  fromPrefix-rev : ∀ {as bs} → Prefix R (reverse as) (reverse bs) →
                   Suffix R as bs
  fromPrefix-rev pre =
    subst₂ (Suffix R)
      (Listₚ.reverse-involutive _)
      (Listₚ.reverse-involutive _)
      (fromPrefix pre)

  toPrefix-rev : ∀ {as bs} → Suffix R as bs →
                 Prefix R (reverse as) (reverse bs)
  toPrefix-rev {as} {bs} s with Suffix.toView s
  ... | Suffix._++_ cs {ds} rs =
    subst (Prefix R (reverse as))
      (sym (Listₚ.reverse-++-commute cs ds))
      (Prefix.fromView (Pw.reverse⁺ rs Prefix.++ reverse cs))

  toPrefix : ∀ {as bs} → Suffix R (reverse as) (reverse bs) →
             Prefix R as bs
  toPrefix suf =
    subst₂ (Prefix R)
      (Listₚ.reverse-involutive _)
      (Listₚ.reverse-involutive _)
      (toPrefix-rev suf)

------------------------------------------------------------------------
-- length

module _ {a b r} {A : Set a} {B : Set b} {R : REL A B r} where

  length-mono : ∀ {as bs} → Suffix R as bs → length as ≤ length bs
  length-mono (here rs)   = ≤-reflexive (Pointwise-length rs)
  length-mono (there suf) = ≤-step (length-mono suf)

  S[as][bs]⇒∣as∣≢1+∣bs∣ : ∀ {as bs} → Suffix R as bs →
                          length as ≢ suc (length bs)
  S[as][bs]⇒∣as∣≢1+∣bs∣ suf eq = <⇒≱ (≤-reflexive (sym eq)) (length-mono suf)

------------------------------------------------------------------------
-- Pointwise conversion

module _ {a b r} {A : Set a} {B : Set b} {R : REL A B r} where

  fromPointwise : Pointwise R ⇒ Suffix R
  fromPointwise = here

  toPointwise : ∀ {as bs} → length as ≡ length bs →
                Suffix R as bs → Pointwise R as bs
  toPointwise eq (here rs)   = rs
  toPointwise eq (there suf) = contradiction eq (S[as][bs]⇒∣as∣≢1+∣bs∣ suf)

------------------------------------------------------------------------
-- Suffix as a partial order

module _ {a b c r s t} {A : Set a} {B : Set b} {C : Set c}
         {R : REL A B r} {S : REL B C s} {T : REL A C t} where

  trans : Trans R S T → Trans (Suffix R) (Suffix S) (Suffix T)
  trans rs⇒t (here rs)    (here ss)       = here (Pw.transitive rs⇒t rs ss)
  trans rs⇒t (here rs)    (there ssuf)    = there (trans rs⇒t (here rs) ssuf)
  trans rs⇒t (there rsuf) ssuf            = trans rs⇒t rsuf (tail ssuf)

module _ {a b e r s} {A : Set a} {B : Set b}
         {R : REL A B r} {S : REL B A s} {E : REL A B e} where

  antisym : Antisym R S E → Antisym (Suffix R) (Suffix S) (Pointwise E)
  antisym rs⇒e rsuf ssuf = Pw.antisymmetric
    rs⇒e
    (toPointwise eq rsuf)
    (toPointwise (sym eq) ssuf)
    where eq = ≤-antisym (length-mono rsuf) (length-mono ssuf)

------------------------------------------------------------------------
-- _++_

module _ {a b r} {A : Set a} {B : Set b} {R : REL A B r} where

  ++⁺ : ∀ {as bs cs ds} → Suffix R as bs → Pointwise R cs ds →
        Suffix R (as ++ cs) (bs ++ ds)
  ++⁺ (here rs)   rs′ = here (Pw.++⁺ rs rs′)
  ++⁺ (there suf) rs′ = there (++⁺ suf rs′)

  ++⁻ : ∀ {as bs cs ds} → length cs ≡ length ds →
        Suffix R (as ++ cs) (bs ++ ds) → Pointwise R cs ds
  ++⁻ {_ ∷ _} {_}      {_}  {_}  eq suf         = ++⁻ eq (tail suf)
  ++⁻ {[]}    {[]}     {_}  {_}  eq suf         = toPointwise eq suf
  ++⁻ {[]}    {b ∷ bs} {_}  {_}  eq (there suf) = ++⁻ eq suf
  ++⁻ {[]}    {b ∷ bs} {cs} {ds} eq (here  rs)  = contradiction (sym eq) (<⇒≢ ds<cs)
    where
    open ≤-Reasoning
    ds<cs : length ds < length cs
    ds<cs = begin-strict
      length ds                   ≤⟨ m≤n+m (length ds) (length bs) ⟩
      length bs + length ds       <⟨ ≤-refl ⟩
      suc (length bs + length ds) ≡⟨ sym $ Listₚ.length-++ (b ∷ bs) ⟩
      length (b ∷ bs ++ ds)       ≡⟨ sym $ Pointwise-length rs ⟩
      length cs                   ∎

------------------------------------------------------------------------
-- map

module _ {a b c d r} {A : Set a} {B : Set b} {C : Set c} {D : Set d}
         {R : REL C D r} where

  map⁺ : ∀ {as bs} (f : A → C) (g : B → D) →
         Suffix (λ a b → R (f a) (g b)) as bs →
         Suffix R (List.map f as) (List.map g bs)
  map⁺ f g (here rs)   = here (Pw.map⁺ f g rs)
  map⁺ f g (there suf) = there (map⁺ f g suf)

  map⁻ : ∀ {as bs} (f : A → C) (g : B → D) →
         Suffix R (List.map f as) (List.map g bs) →
         Suffix (λ a b → R (f a) (g b)) as bs
  map⁻ {as} {b ∷ bs} f g (here rs)   = here (Pw.map⁻ f g rs)
  map⁻ {as} {b ∷ bs} f g (there suf) = there (map⁻ f g suf)
  map⁻ {x ∷ as} {[]} f g suf         = contradiction (length-mono suf) λ()
  map⁻ {[]}     {[]} f g suf         = here []

------------------------------------------------------------------------
-- filter

module _ {a b r p q} {A : Set a} {B : Set b} {R : REL A B r}
         {P : Pred A p} {Q : Pred B q}
         (P? : U.Decidable P) (Q? : U.Decidable Q)
         (P⇒Q : ∀ {a b} → R a b → P a → Q b)
         (Q⇒P : ∀ {a b} → R a b → Q b → P a)
         where

  filter⁺ : ∀ {as bs} → Suffix R as bs →
            Suffix R (filter P? as) (filter Q? bs)
  filter⁺ (here rs) = here (Pw.filter⁺ P? Q? P⇒Q Q⇒P rs)
  filter⁺ (there {a} suf) with does (Q? a)
  ... | true  = there (filter⁺ suf)
  ... | false = filter⁺ suf

------------------------------------------------------------------------
-- replicate

module _ {a b r} {A : Set a} {B : Set b} {R : REL A B r} where

  replicate⁺ : ∀ {m n a b} → m ≤ n → R a b →
               Suffix R (replicate m a) (replicate n b)
  replicate⁺ {a = a} {b = b} m≤n r = repl (≤⇒≤′ m≤n)
    where
    repl : ∀ {m n} → m ≤′ n → Suffix R (replicate m a) (replicate n b)
    repl ≤′-refl       = here (Pw.replicate⁺ r _)
    repl (≤′-step m≤n) = there (repl m≤n)

------------------------------------------------------------------------
-- Irrelevant

module _ {a b r} {A : Set a} {B : Set b} {R : REL A B r} where

  irrelevant : Irrelevant R → Irrelevant (Suffix R)
  irrelevant irr (here  rs)   (here  rs₁)   = P.cong here $ Pw.irrelevant irr rs rs₁
  irrelevant irr (here  rs)   (there rsuf)  = contradiction (Pointwise-length rs) (S[as][bs]⇒∣as∣≢1+∣bs∣ rsuf)
  irrelevant irr (there rsuf) (here  rs)    = contradiction (Pointwise-length rs) (S[as][bs]⇒∣as∣≢1+∣bs∣ rsuf)
  irrelevant irr (there rsuf) (there rsuf₁) = P.cong there $ irrelevant irr rsuf rsuf₁

------------------------------------------------------------------------
-- Decidability

  suffix? : B.Decidable R → B.Decidable (Suffix R)
  suffix? R? as bs = Dec.map′ fromPrefix-rev toPrefix-rev
                   $ Prefixₚ.prefix? R? (reverse as) (reverse bs)
